proof/refine/ARM_HYP/InterruptAcc_R.thy
@@ -63,7 +63,12 @@ lemma setIRQState_invs[wp]:
                         if_unsafe_then_cap'_def ex_cte_cap_to'_def
                         valid_irq_handlers'_def irq_issued'_def
                         cteCaps_of_def valid_irq_masks'_def
-                        bitmapQ_defs valid_queues_no_bitmap_def)
+                        bitmapQ_defs valid_queues_no_bitmap_def split: option.splits)
+   apply (rule conjI, clarsimp)
+   apply (clarsimp simp: irqs_masked'_def ct_not_inQ_def)
+   apply (rule conjI)
+    apply fastforce
+   apply (simp add: ct_idle_or_in_cur_domain'_def tcb_in_cur_domain'_def)
   apply (rule conjI, clarsimp)
   apply (clarsimp simp: irqs_masked'_def ct_not_inQ_def)
   apply (rule conjI)
